Tables/Table/Raw/Join.lean
@@ -35,26 +35,59 @@ def crossJoin (self other : Raw) (h₁ : self.WfColumnSize) (h₂ : other.WfColu
 
   ofRows schema rows.unattach (by grind [Array.mem_unattach])
 
+@[specialize]
+def buildJoinMap {α} [BEq α] [Hashable α] (other : Raw) (h : other.WfColumnSize) (getKey : Row → α) : HashMap α (Array (Fin other.nrows)) :=
+  Nat.fold (init := ∅) other.nrows fun i isLt m =>
+    let key := getKey (other.getRow i isLt h)
+    m.alter key fun
+      | some ns => some (ns.push ⟨i, isLt⟩)
+      | none => some #[⟨i, isLt⟩]
+
 def leftJoin (self other : Raw) (keys : Array String)
     (h₁ : self.WfColumnSize) (h₂ : other.WfColumnSize) : Raw :=
   let schema := self.schema ++ other.schema.selectNotByNames keys
-
-  let otherRowsMap : HashMap Row (Array (Fin other.nrows)) := Nat.fold (init := ∅) other.nrows fun i isLt m =>
-    let row := other.getRow i isLt h₂
-    let keyRow := row.selectByNames keys
-    m.alter keyRow fun
-      | some xs => some (xs.push ⟨i, isLt⟩)
-      | none => some #[⟨i, isLt⟩]
+  let joinMap := other.buildJoinMap h₂ fun row => row.selectByNames keys
 
   let rows : Array { row : Row // row.schema = schema } :=
     Nat.fold (init := #[]) self.nrows fun i isLt rows =>
       let row := self.getRow i isLt h₁
       let keyRow := row.selectByNames keys
-      match otherRowsMap.get? keyRow with
+      match joinMap.get? keyRow with
       | some ns =>
         rows ++ ns.map fun j => ⟨row ++ (other.getRow j.val j.isLt h₂).selectNotByNames keys, by simp [row, schema]⟩
+      | none => rows -- TODO: fill with null values
+
+  ofRows schema rows.unattach (by grind [Array.mem_unattach])
+
+def join {α} [BEq α] [Hashable α] (self other : Raw) (schema : Schema)
+    (getKey₁ : Row → α) (getKey₂ : Row → α)
+    (combine : Row → Row → Row)
+    (h₁ : self.WfColumnSize) (h₂ : other.WfColumnSize)
+    (h₃ : ∀ r₁ r₂, (combine r₁ r₂).schema = schema) : Raw :=
+  let joinMap := other.buildJoinMap h₂ getKey₂
+
+  let rows : Array { row : Row // row.schema = schema } :=
+    Nat.fold (init := #[]) self.nrows fun i isLt rows =>
+      let key := getKey₁ (self.getRow i isLt h₁)
+      match joinMap.get? key with
+      | some ns =>
+        rows ++ ns.map fun j => ⟨combine (self.getRow i isLt h₁) (other.getRow j.val j.isLt h₂), by simp [h₃]⟩
       | none => rows
 
+  ofRows schema rows.unattach (by grind [Array.mem_unattach])
+
+def groupJoin {α} [BEq α] [Hashable α] (self other : Raw) (schema : Schema)
+    (getKey₁ : Row → α) (getKey₂ : Row → α)
+    (combine : Row → Raw → Row)
+    (h₁ : self.WfColumnSize) (h₂ : other.WfColumnSize)
+    (h₃ : ∀ r₁ r₂, (combine r₁ r₂).schema = schema) : Raw :=
+  let joinMap := other.buildJoinMap h₂ getKey₂
+  let rows : Array { row : Row // row.schema = schema } :=
+    Nat.fold (init := #[]) self.nrows fun i isLt rows =>
+      let key := getKey₁ (self.getRow i isLt h₁)
+      match joinMap.get? key with
+      | some ns => rows.push ⟨combine (self.getRow i isLt h₁) (other.selectRows ns h₂), by simp [h₃]⟩
+      | none => rows
   ofRows schema rows.unattach (by grind [Array.mem_unattach])
 
 end Tables.Table.Raw
